theories/theories/utp_boyle.thy
@@ -1,0 +1,36 @@
+theory utp_boyle
+imports utp_base
+begin
+
+abbreviation "k \<equiv> MkPlainP ''k'' True TYPE(real) TYPE('m :: REAL_SORT)"
+abbreviation "p \<equiv> MkPlainP ''p'' True TYPE(real) TYPE('m :: REAL_SORT)"
+abbreviation "V \<equiv> MkPlainP ''V'' True TYPE(real) TYPE('m :: REAL_SORT)"
+
+definition "BH(\<phi>) = `(\<exists> k. \<phi>) \<and> ($k = $p * $V)`"
+
+declare BH_def [eval]
+
+lemma BH_idem: "BH(BH(\<phi>)) = BH(\<phi>)"
+  apply (simp add:BH_def)
+  apply (utp_pred_auto_tac)
+done
+
+lemma BH_example_1:
+  "`($p = \<guillemotleft>10\<guillemotright>) \<and> ($V = \<guillemotleft>5\<guillemotright>) \<and> ($k = \<guillemotleft>50\<guillemotright>)` is BH"
+  by (utp_pred_auto_tac)
+
+lemma DestReal_binding: 
+  "vtype x = RealType \<Longrightarrow>
+   DestReal (\<langle>b(x :=\<^sub>b MkReal n)\<rangle>\<^sub>b x) = n"
+  by (metis MkReal_type REAL_SORT_class.Defined REAL_SORT_class.Inverse binding_upd_apply var_compat_intros(1))
+  
+lemma BH_example_2:
+  "BH(`($p = \<guillemotleft>10\<guillemotright>) \<and> ($V = \<guillemotleft>5\<guillemotright>) \<and> ($k = \<guillemotleft>100\<guillemotright>)`) = 
+      `($p = \<guillemotleft>10\<guillemotright>) \<and> ($V = \<guillemotleft>5\<guillemotright>) \<and> ($k = \<guillemotleft>50\<guillemotright>)`"
+  apply (utp_pred_auto_tac)
+  apply (rule)
+  apply (rule DestReal_binding)
+  apply (metis PVAR_VAR_vtype TypeU_real)
+done
+  
+end
